<?xml version="1.0"?>
<rdf:RDF xmlns="http://ontologies.khaos.uma.es/oulad/"
     xml:base="http://ontologies.khaos.uma.es/oulad/"
     xmlns:owl="http://www.w3.org/2002/07/owl#"
     xmlns:rdf="http://www.w3.org/1999/02/22-rdf-syntax-ns#"
     xmlns:xml="http://www.w3.org/XML/1998/namespace"
     xmlns:xsd="http://www.w3.org/2001/XMLSchema#"
     xmlns:rdfs="http://www.w3.org/2000/01/rdf-schema#">
    <owl:Ontology rdf:about="http://ontologies.khaos.uma.es/oulad/">
        <rdfs:label>OULAD</rdfs:label>
    </owl:Ontology>
    


    <!-- 
    ///////////////////////////////////////////////////////////////////////////////////////
    //
    // Object Properties
    //
    ///////////////////////////////////////////////////////////////////////////////////////
     -->


    


    <!-- http://ontologies.khaos.uma.es/oulad/assessment_has_course -->


    <owl:ObjectProperty rdf:about="http://ontologies.khaos.uma.es/oulad/assessment_has_course">
        <rdfs:domain rdf:resource="http://ontologies.khaos.uma.es/oulad/Assessments"/>
        <rdfs:range rdf:resource="http://ontologies.khaos.uma.es/oulad/Courses"/>
        <rdfs:comment xml:lang="es">Identification code of the module and presentation, to which the assessment belongs.</rdfs:comment>
        <rdfs:label xml:lang="es">assessment_has_course</rdfs:label>
    </owl:ObjectProperty>
    


    <!-- http://ontologies.khaos.uma.es/oulad/student_assessment_has_assessment -->


    <owl:ObjectProperty rdf:about="http://ontologies.khaos.uma.es/oulad/student_assessment_has_assessment">
        <rdfs:domain rdf:resource="http://ontologies.khaos.uma.es/oulad/StudentAssessment"/>
        <rdfs:range rdf:resource="http://ontologies.khaos.uma.es/oulad/Assessments"/>
        <rdfs:label xml:lang="es">The identification of the assessment.</rdfs:label>
        <rdfs:label xml:lang="es">student_assessment_has_assessment</rdfs:label>
    </owl:ObjectProperty>
    


    <!-- http://ontologies.khaos.uma.es/oulad/student_assessment_has_student -->


    <owl:ObjectProperty rdf:about="http://ontologies.khaos.uma.es/oulad/student_assessment_has_student">
        <rdfs:domain rdf:resource="http://ontologies.khaos.uma.es/oulad/StudentAssessment"/>
        <rdfs:range rdf:resource="http://ontologies.khaos.uma.es/oulad/StudentInfo"/>
        <rdfs:comment xml:lang="es">A identification for the student.</rdfs:comment>
        <rdfs:label xml:lang="es">student_assessment_has_student</rdfs:label>
    </owl:ObjectProperty>
    


    <!-- http://ontologies.khaos.uma.es/oulad/student_info_has_course -->


    <owl:ObjectProperty rdf:about="http://ontologies.khaos.uma.es/oulad/student_info_has_course">
        <rdfs:domain rdf:resource="http://ontologies.khaos.uma.es/oulad/StudentInfo"/>
        <rdfs:range rdf:resource="http://ontologies.khaos.uma.es/oulad/Courses"/>
        <rdfs:comment xml:lang="es">An identification for a module and presentation on which the student is registered.</rdfs:comment>
        <rdfs:label xml:lang="es">student_info_has_course</rdfs:label>
    </owl:ObjectProperty>
    


    <!-- http://ontologies.khaos.uma.es/oulad/student_registration_has_course -->


    <owl:ObjectProperty rdf:about="http://ontologies.khaos.uma.es/oulad/student_registration_has_course">
        <rdfs:subPropertyOf rdf:resource="http://www.w3.org/2002/07/owl#topObjectProperty"/>
        <rdfs:domain rdf:resource="http://ontologies.khaos.uma.es/oulad/StudentRegistration"/>
        <rdfs:range rdf:resource="http://ontologies.khaos.uma.es/oulad/Courses"/>
        <rdfs:comment xml:lang="es">The identification code of the module presentation.</rdfs:comment>
        <rdfs:label xml:lang="es">student_registration_has_course</rdfs:label>
    </owl:ObjectProperty>
    


    <!-- http://ontologies.khaos.uma.es/oulad/student_registration_has_student_info -->


    <owl:ObjectProperty rdf:about="http://ontologies.khaos.uma.es/oulad/student_registration_has_student_info">
        <rdfs:domain rdf:resource="http://ontologies.khaos.uma.es/oulad/StudentRegistration"/>
        <rdfs:range rdf:resource="http://ontologies.khaos.uma.es/oulad/StudentInfo"/>
        <rdfs:comment xml:lang="es">A identification for the student.</rdfs:comment>
        <rdfs:label xml:lang="es">student_registration_has_student_info</rdfs:label>
    </owl:ObjectProperty>
    


    <!-- http://ontologies.khaos.uma.es/oulad/student_vle_has_student_info -->


    <owl:ObjectProperty rdf:about="http://ontologies.khaos.uma.es/oulad/student_vle_has_student_info">
        <rdfs:domain rdf:resource="http://ontologies.khaos.uma.es/oulad/StudentVle"/>
        <rdfs:range rdf:resource="http://ontologies.khaos.uma.es/oulad/StudentInfo"/>
        <rdfs:comment xml:lang="es">A identification for the student info.</rdfs:comment>
        <rdfs:label xml:lang="es">student_vle_has_student_info</rdfs:label>
    </owl:ObjectProperty>
    


    <!-- http://ontologies.khaos.uma.es/oulad/student_vle_has_vle -->


    <owl:ObjectProperty rdf:about="http://ontologies.khaos.uma.es/oulad/student_vle_has_vle">
        <rdfs:domain rdf:resource="http://ontologies.khaos.uma.es/oulad/StudentVle"/>
        <rdfs:range rdf:resource="http://ontologies.khaos.uma.es/oulad/Vle"/>
        <rdfs:comment xml:lang="es">An identification for the VLE material.</rdfs:comment>
        <rdfs:label xml:lang="es">student_vle_has_vle</rdfs:label>
    </owl:ObjectProperty>
    


    <!-- http://ontologies.khaos.uma.es/oulad/vle_has_course -->


    <owl:ObjectProperty rdf:about="http://ontologies.khaos.uma.es/oulad/vle_has_course">
        <rdfs:domain rdf:resource="http://ontologies.khaos.uma.es/oulad/Vle"/>
        <rdfs:range rdf:resource="http://ontologies.khaos.uma.es/oulad/Courses"/>
        <rdfs:comment xml:lang="es">An identification code for module and presentation.</rdfs:comment>
        <rdfs:label xml:lang="es">vle_has_course</rdfs:label>
    </owl:ObjectProperty>
    


    <!-- 
    ///////////////////////////////////////////////////////////////////////////////////////
    //
    // Data properties
    //
    ///////////////////////////////////////////////////////////////////////////////////////
     -->


    


    <!-- http://ontologies.khaos.uma.es/oulad/activity_type -->


    <owl:DatatypeProperty rdf:about="http://ontologies.khaos.uma.es/oulad/activity_type">
        <rdfs:domain rdf:resource="http://ontologies.khaos.uma.es/oulad/Vle"/>
        <rdfs:range rdf:resource="http://www.w3.org/2001/XMLSchema#string"/>
        <rdfs:comment xml:lang="en">The role associated with the module material.</rdfs:comment>
        <rdfs:label xml:lang="en">activity_type</rdfs:label>
    </owl:DatatypeProperty>
    


    <!-- http://ontologies.khaos.uma.es/oulad/age_band -->


    <owl:DatatypeProperty rdf:about="http://ontologies.khaos.uma.es/oulad/age_band">
        <rdfs:domain rdf:resource="http://ontologies.khaos.uma.es/oulad/StudentInfo"/>
        <rdfs:range rdf:resource="http://www.w3.org/2001/XMLSchema#string"/>
        <rdfs:comment xml:lang="en">Band of the student’s age.</rdfs:comment>
        <rdfs:label xml:lang="en">age_band</rdfs:label>
    </owl:DatatypeProperty>
    


    <!-- http://ontologies.khaos.uma.es/oulad/assessment_type -->


    <owl:DatatypeProperty rdf:about="http://ontologies.khaos.uma.es/oulad/assessment_type">
        <rdfs:domain rdf:resource="http://ontologies.khaos.uma.es/oulad/Assessments"/>
        <rdfs:range rdf:resource="http://www.w3.org/2001/XMLSchema#string"/>
        <rdfs:comment xml:lang="en">Type of assessment. Three types of assessments exist: Tutor Marked Assessment (TMA), Computer Marked Assessment (CMA) and Final Exam (Exam).</rdfs:comment>
        <rdfs:label xml:lang="en">assessment_type</rdfs:label>
    </owl:DatatypeProperty>
    


    <!-- http://ontologies.khaos.uma.es/oulad/code_module -->


    <owl:DatatypeProperty rdf:about="http://ontologies.khaos.uma.es/oulad/code_module">
        <rdfs:domain rdf:resource="http://ontologies.khaos.uma.es/oulad/Courses"/>
        <rdfs:range rdf:resource="http://www.w3.org/2001/XMLSchema#string"/>
        <rdfs:comment xml:lang="en">Code name of the module, which serves as the identifier.</rdfs:comment>
        <rdfs:label xml:lang="en">code_module</rdfs:label>
    </owl:DatatypeProperty>
    


    <!-- http://ontologies.khaos.uma.es/oulad/code_presentation -->


    <owl:DatatypeProperty rdf:about="http://ontologies.khaos.uma.es/oulad/code_presentation">
        <rdfs:domain rdf:resource="http://ontologies.khaos.uma.es/oulad/Courses"/>
        <rdfs:range rdf:resource="http://www.w3.org/2001/XMLSchema#string"/>
        <rdfs:comment xml:lang="en">Code name of the presentation. It consists of the year and “B” for the presentation starting in February and “J” for the presentation starting in October.</rdfs:comment>
        <rdfs:label xml:lang="en">code_presentation</rdfs:label>
    </owl:DatatypeProperty>
    


    <!-- http://ontologies.khaos.uma.es/oulad/date -->


    <owl:DatatypeProperty rdf:about="http://ontologies.khaos.uma.es/oulad/date">
        <rdfs:domain rdf:resource="http://ontologies.khaos.uma.es/oulad/Assessments"/>
        <rdfs:range rdf:resource="http://www.w3.org/2001/XMLSchema#dateTime"/>
        <rdfs:comment xml:lang="en">Information about the final submission date of the assessment calculated as the number of days since the start of the module-presentation.</rdfs:comment>
        <rdfs:label xml:lang="en">date</rdfs:label>
    </owl:DatatypeProperty>
    


    <!-- http://ontologies.khaos.uma.es/oulad/date_registration -->


    <owl:DatatypeProperty rdf:about="http://ontologies.khaos.uma.es/oulad/date_registration">
        <rdfs:domain rdf:resource="http://ontologies.khaos.uma.es/oulad/StudentRegistration"/>
        <rdfs:range rdf:resource="http://www.w3.org/2001/XMLSchema#dateTime"/>
        <rdfs:comment xml:lang="en">The date of student’s registration on the module presentation.</rdfs:comment>
        <rdfs:label xml:lang="en">date_registration</rdfs:label>
    </owl:DatatypeProperty>
    


    <!-- http://ontologies.khaos.uma.es/oulad/date_student_vle -->


    <owl:DatatypeProperty rdf:about="http://ontologies.khaos.uma.es/oulad/date_student_vle">
        <rdfs:domain rdf:resource="http://ontologies.khaos.uma.es/oulad/StudentVle"/>
        <rdfs:range rdf:resource="http://www.w3.org/2001/XMLSchema#dateTime"/>
        <rdfs:comment xml:lang="en">The date of student’s interaction with the material.</rdfs:comment>
        <rdfs:label xml:lang="en">date_student_vle</rdfs:label>
    </owl:DatatypeProperty>
    


    <!-- http://ontologies.khaos.uma.es/oulad/date_submitted -->


    <owl:DatatypeProperty rdf:about="http://ontologies.khaos.uma.es/oulad/date_submitted">
        <rdfs:domain rdf:resource="http://ontologies.khaos.uma.es/oulad/StudentAssessment"/>
        <rdfs:range rdf:resource="http://www.w3.org/2001/XMLSchema#dateTime"/>
        <rdfs:comment xml:lang="en">The date of student submission.</rdfs:comment>
        <rdfs:label xml:lang="en">date_submitted</rdfs:label>
    </owl:DatatypeProperty>
    


    <!-- http://ontologies.khaos.uma.es/oulad/date_unregistration -->


    <owl:DatatypeProperty rdf:about="http://ontologies.khaos.uma.es/oulad/date_unregistration">
        <rdfs:domain rdf:resource="http://ontologies.khaos.uma.es/oulad/StudentRegistration"/>
        <rdfs:range rdf:resource="http://www.w3.org/2001/XMLSchema#dateTime"/>
        <rdfs:comment xml:lang="en">Date of student unregistration from the module presentation. Students, who completed the course have this field empty. Students who unregistered have Withdrawal as the value of the final_result.</rdfs:comment>
        <rdfs:label xml:lang="en">date_unregistration</rdfs:label>
    </owl:DatatypeProperty>
    


    <!-- http://ontologies.khaos.uma.es/oulad/disability -->


    <owl:DatatypeProperty rdf:about="http://ontologies.khaos.uma.es/oulad/disability">
        <rdfs:domain rdf:resource="http://ontologies.khaos.uma.es/oulad/StudentInfo"/>
        <rdfs:range rdf:resource="http://www.w3.org/2001/XMLSchema#string"/>
        <rdfs:comment xml:lang="en">Indicates whether the student has declared a disability.</rdfs:comment>
        <rdfs:label xml:lang="en">disability</rdfs:label>
    </owl:DatatypeProperty>
    


    <!-- http://ontologies.khaos.uma.es/oulad/final_result -->


    <owl:DatatypeProperty rdf:about="http://ontologies.khaos.uma.es/oulad/final_result">
        <rdfs:domain rdf:resource="http://ontologies.khaos.uma.es/oulad/StudentInfo"/>
        <rdfs:range rdf:resource="http://www.w3.org/2001/XMLSchema#string"/>
        <rdfs:comment xml:lang="en">Student’s final result in the module-presentation.</rdfs:comment>
        <rdfs:label xml:lang="en">final_result</rdfs:label>
    </owl:DatatypeProperty>
    


    <!-- http://ontologies.khaos.uma.es/oulad/gender -->


    <owl:DatatypeProperty rdf:about="http://ontologies.khaos.uma.es/oulad/gender">
        <rdfs:domain rdf:resource="http://ontologies.khaos.uma.es/oulad/StudentInfo"/>
        <rdfs:range rdf:resource="http://www.w3.org/2001/XMLSchema#string"/>
        <rdfs:comment xml:lang="en">The student’s gender.</rdfs:comment>
        <rdfs:label xml:lang="en">gender</rdfs:label>
    </owl:DatatypeProperty>
    


    <!-- http://ontologies.khaos.uma.es/oulad/highest_education -->


    <owl:DatatypeProperty rdf:about="http://ontologies.khaos.uma.es/oulad/highest_education">
        <rdfs:domain rdf:resource="http://ontologies.khaos.uma.es/oulad/StudentInfo"/>
        <rdfs:range rdf:resource="http://www.w3.org/2001/XMLSchema#string"/>
        <rdfs:comment xml:lang="en">Highest student education level on entry to the module presentation.</rdfs:comment>
        <rdfs:label xml:lang="en">highest_education</rdfs:label>
    </owl:DatatypeProperty>
    


    <!-- http://ontologies.khaos.uma.es/oulad/id_assessment -->


    <owl:DatatypeProperty rdf:about="http://ontologies.khaos.uma.es/oulad/id_assessment">
        <rdfs:domain rdf:resource="http://ontologies.khaos.uma.es/oulad/Assessments"/>
        <rdfs:range rdf:resource="http://www.w3.org/2001/XMLSchema#integer"/>
        <rdfs:comment xml:lang="en">Identification number of the assessment.</rdfs:comment>
        <rdfs:label xml:lang="en">id_assessment</rdfs:label>
    </owl:DatatypeProperty>
    


    <!-- http://ontologies.khaos.uma.es/oulad/id_site -->


    <owl:DatatypeProperty rdf:about="http://ontologies.khaos.uma.es/oulad/id_site">
        <rdfs:domain rdf:resource="http://ontologies.khaos.uma.es/oulad/Vle"/>
        <rdfs:comment xml:lang="en">An identification number of the material.</rdfs:comment>
        <rdfs:label xml:lang="en">id_site</rdfs:label>
    </owl:DatatypeProperty>
    


    <!-- http://ontologies.khaos.uma.es/oulad/id_student -->


    <owl:DatatypeProperty rdf:about="http://ontologies.khaos.uma.es/oulad/id_student">
        <rdfs:domain rdf:resource="http://ontologies.khaos.uma.es/oulad/StudentInfo"/>
        <rdfs:range rdf:resource="http://www.w3.org/2001/XMLSchema#integer"/>
        <rdfs:comment xml:lang="en">A unique identification number for the student.</rdfs:comment>
        <rdfs:label xml:lang="en">id_student</rdfs:label>
    </owl:DatatypeProperty>
    


    <!-- http://ontologies.khaos.uma.es/oulad/imd_band -->


    <owl:DatatypeProperty rdf:about="http://ontologies.khaos.uma.es/oulad/imd_band">
        <rdfs:domain rdf:resource="http://ontologies.khaos.uma.es/oulad/StudentInfo"/>
        <rdfs:range rdf:resource="http://www.w3.org/2001/XMLSchema#string"/>
        <rdfs:comment xml:lang="en">Specifies the Index of Multiple Depravation band of the place where the student lived during the module-presentation.</rdfs:comment>
        <rdfs:label xml:lang="en">imd_band</rdfs:label>
    </owl:DatatypeProperty>
    


    <!-- http://ontologies.khaos.uma.es/oulad/is_banked -->


    <owl:DatatypeProperty rdf:about="http://ontologies.khaos.uma.es/oulad/is_banked">
        <rdfs:domain rdf:resource="http://ontologies.khaos.uma.es/oulad/StudentAssessment"/>
        <rdfs:range rdf:resource="http://www.w3.org/2001/XMLSchema#string"/>
        <rdfs:comment xml:lang="en">A status flag indicating that the assessment result has been transferred from a previous presentation.</rdfs:comment>
        <rdfs:label xml:lang="en">is_banked</rdfs:label>
    </owl:DatatypeProperty>
    


    <!-- http://ontologies.khaos.uma.es/oulad/length -->


    <owl:DatatypeProperty rdf:about="http://ontologies.khaos.uma.es/oulad/length">
        <rdfs:domain rdf:resource="http://ontologies.khaos.uma.es/oulad/Courses"/>
        <rdfs:range rdf:resource="http://www.w3.org/2001/XMLSchema#integer"/>
        <rdfs:comment xml:lang="en">Length of the module-presentation in days.</rdfs:comment>
        <rdfs:label xml:lang="en">length</rdfs:label>
    </owl:DatatypeProperty>
    


    <!-- http://ontologies.khaos.uma.es/oulad/num_of_prev_attempts -->


    <owl:DatatypeProperty rdf:about="http://ontologies.khaos.uma.es/oulad/num_of_prev_attempts">
        <rdfs:domain rdf:resource="http://ontologies.khaos.uma.es/oulad/StudentInfo"/>
        <rdfs:range rdf:resource="http://www.w3.org/2001/XMLSchema#integer"/>
        <rdfs:comment xml:lang="en">The number times the student has attempted this module.</rdfs:comment>
        <rdfs:label xml:lang="en">num_of_prev_attempts</rdfs:label>
    </owl:DatatypeProperty>
    


    <!-- http://ontologies.khaos.uma.es/oulad/region -->


    <owl:DatatypeProperty rdf:about="http://ontologies.khaos.uma.es/oulad/region">
        <rdfs:range rdf:resource="http://www.w3.org/2001/XMLSchema#string"/>
        <rdfs:comment xml:lang="en">Identifies the geographic region, where the student lived while taking the module-presentation.</rdfs:comment>
        <rdfs:label xml:lang="en">region</rdfs:label>
    </owl:DatatypeProperty>
    


    <!-- http://ontologies.khaos.uma.es/oulad/score -->


    <owl:DatatypeProperty rdf:about="http://ontologies.khaos.uma.es/oulad/score">
        <rdfs:domain rdf:resource="http://ontologies.khaos.uma.es/oulad/StudentAssessment"/>
        <rdfs:range rdf:resource="http://www.w3.org/2001/XMLSchema#float"/>
        <rdfs:comment xml:lang="en">The student’s score in this assessment. The range is from 0 to 100. The score lower than 40 is interpreted as Fail. The marks are in the range from 0 to 100.</rdfs:comment>
        <rdfs:label xml:lang="en">score</rdfs:label>
    </owl:DatatypeProperty>
    


    <!-- http://ontologies.khaos.uma.es/oulad/studied_credits -->


    <owl:DatatypeProperty rdf:about="http://ontologies.khaos.uma.es/oulad/studied_credits">
        <rdfs:domain rdf:resource="http://ontologies.khaos.uma.es/oulad/StudentInfo"/>
        <rdfs:range rdf:resource="http://www.w3.org/2001/XMLSchema#integer"/>
        <rdfs:comment xml:lang="en">The total number of credits for the modules the student is currently studying.</rdfs:comment>
        <rdfs:label xml:lang="en">studied_credits</rdfs:label>
    </owl:DatatypeProperty>
    


    <!-- http://ontologies.khaos.uma.es/oulad/sum_click -->


    <owl:DatatypeProperty rdf:about="http://ontologies.khaos.uma.es/oulad/sum_click">
        <rdfs:domain rdf:resource="http://ontologies.khaos.uma.es/oulad/StudentVle"/>
        <rdfs:range rdf:resource="http://www.w3.org/2001/XMLSchema#integer"/>
        <rdfs:comment xml:lang="en">The number of times a student interacts with the material in that day.</rdfs:comment>
        <rdfs:label xml:lang="en">sum_click</rdfs:label>
    </owl:DatatypeProperty>
    


    <!-- http://ontologies.khaos.uma.es/oulad/week_from -->


    <owl:DatatypeProperty rdf:about="http://ontologies.khaos.uma.es/oulad/week_from">
        <rdfs:domain rdf:resource="http://ontologies.khaos.uma.es/oulad/Vle"/>
        <rdfs:range rdf:resource="http://www.w3.org/2001/XMLSchema#integer"/>
        <rdfs:comment xml:lang="en">The week from which the material is planned to be used.</rdfs:comment>
        <rdfs:label xml:lang="en">week_from</rdfs:label>
    </owl:DatatypeProperty>
    


    <!-- http://ontologies.khaos.uma.es/oulad/week_to -->


    <owl:DatatypeProperty rdf:about="http://ontologies.khaos.uma.es/oulad/week_to">
        <rdfs:domain rdf:resource="http://ontologies.khaos.uma.es/oulad/Vle"/>
        <rdfs:range rdf:resource="http://www.w3.org/2001/XMLSchema#integer"/>
        <rdfs:comment xml:lang="en">Week until which the material is planned to be used.</rdfs:comment>
        <rdfs:label xml:lang="en">week_to</rdfs:label>
    </owl:DatatypeProperty>
    


    <!-- http://ontologies.khaos.uma.es/oulad/weight -->


    <owl:DatatypeProperty rdf:about="http://ontologies.khaos.uma.es/oulad/weight">
        <rdfs:domain rdf:resource="http://ontologies.khaos.uma.es/oulad/Assessments"/>
        <rdfs:range rdf:resource="http://www.w3.org/2001/XMLSchema#integer"/>
        <rdfs:comment xml:lang="en">Weight of the assessment in %. Typically, Exams are treated separately and have the weight 100%; the sum of all other assessments is 100%</rdfs:comment>
        <rdfs:label xml:lang="en">weight</rdfs:label>
    </owl:DatatypeProperty>
    


    <!-- 
    ///////////////////////////////////////////////////////////////////////////////////////
    //
    // Classes
    //
    ///////////////////////////////////////////////////////////////////////////////////////
     -->


    


    <!-- http://ontologies.khaos.uma.es/oulad/Assessments -->


    <owl:Class rdf:about="http://ontologies.khaos.uma.es/oulad/Assessments">
        <rdfs:comment xml:lang="en">This class models the information about assessments in module-presentations. Usually, every presentation has a number of assessments followed by the final exam.</rdfs:comment>
        <rdfs:label xml:lang="en">Assessments</rdfs:label>
    </owl:Class>
    


    <!-- http://ontologies.khaos.uma.es/oulad/Courses -->


    <owl:Class rdf:about="http://ontologies.khaos.uma.es/oulad/Courses">
        <rdfs:comment xml:lang="en">This class models all available modules and their presentations.</rdfs:comment>
        <rdfs:label xml:lang="en">Courses</rdfs:label>
    </owl:Class>
    


    <!-- http://ontologies.khaos.uma.es/oulad/StudentAssessment -->


    <owl:Class rdf:about="http://ontologies.khaos.uma.es/oulad/StudentAssessment">
        <rdfs:comment xml:lang="en">This class models the results of students’ assessments. If the student does not submit the assessment, no result is recorded.</rdfs:comment>
        <rdfs:label xml:lang="en">Student Assessment</rdfs:label>
    </owl:Class>
    


    <!-- http://ontologies.khaos.uma.es/oulad/StudentInfo -->


    <owl:Class rdf:about="http://ontologies.khaos.uma.es/oulad/StudentInfo">
        <rdfs:comment xml:lang="en">This class models the demographic information about the students together with their results.</rdfs:comment>
        <rdfs:label xml:lang="en">Student Info</rdfs:label>
    </owl:Class>
    


    <!-- http://ontologies.khaos.uma.es/oulad/StudentRegistration -->


    <owl:Class rdf:about="http://ontologies.khaos.uma.es/oulad/StudentRegistration">
        <rdfs:comment xml:lang="en">This class models the information about the time when the student registered for the module presentation.</rdfs:comment>
        <rdfs:label xml:lang="en">Student Registration</rdfs:label>
    </owl:Class>
    


    <!-- http://ontologies.khaos.uma.es/oulad/StudentVle -->


    <owl:Class rdf:about="http://ontologies.khaos.uma.es/oulad/StudentVle">
        <rdfs:comment xml:lang="en">This class models the information about each student’s interactions with the materials in the VLE.</rdfs:comment>
        <rdfs:label xml:lang="en">Student Vle</rdfs:label>
    </owl:Class>
    


    <!-- http://ontologies.khaos.uma.es/oulad/Vle -->


    <owl:Class rdf:about="http://ontologies.khaos.uma.es/oulad/Vle">
        <rdfs:comment xml:lang="en">This class models the information about the available materials in the VLE. Typically these are html pages, pdf files, etc. Students have access to these materials online and their interactions with the materials are recorded.</rdfs:comment>
        <rdfs:label xml:lang="en">Vle</rdfs:label>
    </owl:Class>
</rdf:RDF>



<!-- Generated by the OWL API (version 5.1.18) https://github.com/owlcs/owlapi/ -->


