@prefix : <http://ontologies.khaos.uma.es/oulad/> .
@prefix owl: <http://www.w3.org/2002/07/owl#> .
@prefix rdf: <http://www.w3.org/1999/02/22-rdf-syntax-ns#> .
@prefix xml: <http://www.w3.org/XML/1998/namespace> .
@prefix xsd: <http://www.w3.org/2001/XMLSchema#> .
@prefix rdfs: <http://www.w3.org/2000/01/rdf-schema#> .
@base <http://ontologies.khaos.uma.es/oulad/> .

<http://ontologies.khaos.uma.es/oulad/> rdf:type owl:Ontology ;
                                         rdfs:label "OULAD" .

#################################################################
#    Object Properties
#################################################################

###  http://ontologies.khaos.uma.es/oulad/assessment_has_course
:assessment_has_course rdf:type owl:ObjectProperty ;
                       rdfs:domain :Assessments ;
                       rdfs:range :Courses ;
                       rdfs:comment "Identification code of the module and presentation, to which the assessment belongs."@es ;
                       rdfs:label "assessment_has_course"@es .


###  http://ontologies.khaos.uma.es/oulad/student_assessment_has_assessment
:student_assessment_has_assessment rdf:type owl:ObjectProperty ;
                                   rdfs:domain :StudentAssessment ;
                                   rdfs:range :Assessments ;
                                   rdfs:label "The identification of the assessment."@es ,
                                              "student_assessment_has_assessment"@es .


###  http://ontologies.khaos.uma.es/oulad/student_assessment_has_student
:student_assessment_has_student rdf:type owl:ObjectProperty ;
                                rdfs:domain :StudentAssessment ;
                                rdfs:range :StudentInfo ;
                                rdfs:comment "A identification for the student."@es ;
                                rdfs:label "student_assessment_has_student"@es .


###  http://ontologies.khaos.uma.es/oulad/student_info_has_course
:student_info_has_course rdf:type owl:ObjectProperty ;
                         rdfs:domain :StudentInfo ;
                         rdfs:range :Courses ;
                         rdfs:comment "An identification for a module and presentation on which the student is registered."@es ;
                         rdfs:label "student_info_has_course"@es .


###  http://ontologies.khaos.uma.es/oulad/student_registration_has_course
:student_registration_has_course rdf:type owl:ObjectProperty ;
                                 rdfs:subPropertyOf owl:topObjectProperty ;
                                 rdfs:domain :StudentRegistration ;
                                 rdfs:range :Courses ;
                                 rdfs:comment "The identification code of the module presentation."@es ;
                                 rdfs:label "student_registration_has_course"@es .


###  http://ontologies.khaos.uma.es/oulad/student_registration_has_student_info
:student_registration_has_student_info rdf:type owl:ObjectProperty ;
                                       rdfs:domain :StudentRegistration ;
                                       rdfs:range :StudentInfo ;
                                       rdfs:comment "A identification for the student."@es ;
                                       rdfs:label "student_registration_has_student_info"@es .


###  http://ontologies.khaos.uma.es/oulad/student_vle_has_student_info
:student_vle_has_student_info rdf:type owl:ObjectProperty ;
                              rdfs:domain :StudentVle ;
                              rdfs:range :StudentInfo ;
                              rdfs:comment "A identification for the student info."@es ;
                              rdfs:label "student_vle_has_student_info"@es .


###  http://ontologies.khaos.uma.es/oulad/student_vle_has_vle
:student_vle_has_vle rdf:type owl:ObjectProperty ;
                     rdfs:domain :StudentVle ;
                     rdfs:range :Vle ;
                     rdfs:comment "An identification for the VLE material."@es ;
                     rdfs:label "student_vle_has_vle"@es .


###  http://ontologies.khaos.uma.es/oulad/vle_has_course
:vle_has_course rdf:type owl:ObjectProperty ;
                rdfs:domain :Vle ;
                rdfs:range :Courses ;
                rdfs:comment "An identification code for module and presentation."@es ;
                rdfs:label "vle_has_course"@es .


#################################################################
#    Data properties
#################################################################

###  http://ontologies.khaos.uma.es/oulad/activity_type
:activity_type rdf:type owl:DatatypeProperty ;
               rdfs:domain :Vle ;
               rdfs:range xsd:string ;
               rdfs:comment "The role associated with the module material."@en ;
               rdfs:label "activity_type"@en .


###  http://ontologies.khaos.uma.es/oulad/age_band
:age_band rdf:type owl:DatatypeProperty ;
          rdfs:domain :StudentInfo ;
          rdfs:range xsd:string ;
          rdfs:comment "Band of the student’s age."@en ;
          rdfs:label "age_band"@en .


###  http://ontologies.khaos.uma.es/oulad/assessment_type
:assessment_type rdf:type owl:DatatypeProperty ;
                 rdfs:domain :Assessments ;
                 rdfs:range xsd:string ;
                 rdfs:comment "Type of assessment. Three types of assessments exist: Tutor Marked Assessment (TMA), Computer Marked Assessment (CMA) and Final Exam (Exam)."@en ;
                 rdfs:label "assessment_type"@en .


###  http://ontologies.khaos.uma.es/oulad/code_module
:code_module rdf:type owl:DatatypeProperty ;
             rdfs:domain :Courses ;
             rdfs:range xsd:string ;
             rdfs:comment "Code name of the module, which serves as the identifier."@en ;
             rdfs:label "code_module"@en .


###  http://ontologies.khaos.uma.es/oulad/code_presentation
:code_presentation rdf:type owl:DatatypeProperty ;
                   rdfs:domain :Courses ;
                   rdfs:range xsd:string ;
                   rdfs:comment "Code name of the presentation. It consists of the year and “B” for the presentation starting in February and “J” for the presentation starting in October."@en ;
                   rdfs:label "code_presentation"@en .


###  http://ontologies.khaos.uma.es/oulad/date
:date rdf:type owl:DatatypeProperty ;
      rdfs:domain :Assessments ;
      rdfs:range xsd:dateTime ;
      rdfs:comment "Information about the final submission date of the assessment calculated as the number of days since the start of the module-presentation."@en ;
      rdfs:label "date"@en .


###  http://ontologies.khaos.uma.es/oulad/date_registration
:date_registration rdf:type owl:DatatypeProperty ;
                   rdfs:domain :StudentRegistration ;
                   rdfs:range xsd:dateTime ;
                   rdfs:comment "The date of student’s registration on the module presentation."@en ;
                   rdfs:label "date_registration"@en .


###  http://ontologies.khaos.uma.es/oulad/date_student_vle
:date_student_vle rdf:type owl:DatatypeProperty ;
                  rdfs:domain :StudentVle ;
                  rdfs:range xsd:dateTime ;
                  rdfs:comment "The date of student’s interaction with the material."@en ;
                  rdfs:label "date_student_vle"@en .


###  http://ontologies.khaos.uma.es/oulad/date_submitted
:date_submitted rdf:type owl:DatatypeProperty ;
                rdfs:domain :StudentAssessment ;
                rdfs:range xsd:dateTime ;
                rdfs:comment "The date of student submission."@en ;
                rdfs:label "date_submitted"@en .


###  http://ontologies.khaos.uma.es/oulad/date_unregistration
:date_unregistration rdf:type owl:DatatypeProperty ;
                     rdfs:domain :StudentRegistration ;
                     rdfs:range xsd:dateTime ;
                     rdfs:comment "Date of student unregistration from the module presentation. Students, who completed the course have this field empty. Students who unregistered have Withdrawal as the value of the final_result."@en ;
                     rdfs:label "date_unregistration"@en .


###  http://ontologies.khaos.uma.es/oulad/disability
:disability rdf:type owl:DatatypeProperty ;
            rdfs:domain :StudentInfo ;
            rdfs:range xsd:string ;
            rdfs:comment "Indicates whether the student has declared a disability."@en ;
            rdfs:label "disability"@en .


###  http://ontologies.khaos.uma.es/oulad/final_result
:final_result rdf:type owl:DatatypeProperty ;
              rdfs:domain :StudentInfo ;
              rdfs:range xsd:string ;
              rdfs:comment "Student’s final result in the module-presentation."@en ;
              rdfs:label "final_result"@en .


###  http://ontologies.khaos.uma.es/oulad/gender
:gender rdf:type owl:DatatypeProperty ;
        rdfs:domain :StudentInfo ;
        rdfs:range xsd:string ;
        rdfs:comment "The student’s gender."@en ;
        rdfs:label "gender"@en .


###  http://ontologies.khaos.uma.es/oulad/highest_education
:highest_education rdf:type owl:DatatypeProperty ;
                   rdfs:domain :StudentInfo ;
                   rdfs:range xsd:string ;
                   rdfs:comment "Highest student education level on entry to the module presentation."@en ;
                   rdfs:label "highest_education"@en .


###  http://ontologies.khaos.uma.es/oulad/id_assessment
:id_assessment rdf:type owl:DatatypeProperty ;
               rdfs:domain :Assessments ;
               rdfs:range xsd:integer ;
               rdfs:comment "Identification number of the assessment."@en ;
               rdfs:label "id_assessment"@en .


###  http://ontologies.khaos.uma.es/oulad/id_site
:id_site rdf:type owl:DatatypeProperty ;
         rdfs:domain :Vle ;
         rdfs:comment "An identification number of the material."@en ;
         rdfs:label "id_site"@en .


###  http://ontologies.khaos.uma.es/oulad/id_student
:id_student rdf:type owl:DatatypeProperty ;
            rdfs:domain :StudentInfo ;
            rdfs:range xsd:integer ;
            rdfs:comment "A unique identification number for the student."@en ;
            rdfs:label "id_student"@en .


###  http://ontologies.khaos.uma.es/oulad/imd_band
:imd_band rdf:type owl:DatatypeProperty ;
          rdfs:domain :StudentInfo ;
          rdfs:range xsd:string ;
          rdfs:comment "Specifies the Index of Multiple Depravation band of the place where the student lived during the module-presentation."@en ;
          rdfs:label "imd_band"@en .


###  http://ontologies.khaos.uma.es/oulad/is_banked
:is_banked rdf:type owl:DatatypeProperty ;
           rdfs:domain :StudentAssessment ;
           rdfs:range xsd:string ;
           rdfs:comment "A status flag indicating that the assessment result has been transferred from a previous presentation."@en ;
           rdfs:label "is_banked"@en .


###  http://ontologies.khaos.uma.es/oulad/length
:length rdf:type owl:DatatypeProperty ;
        rdfs:domain :Courses ;
        rdfs:range xsd:integer ;
        rdfs:comment "Length of the module-presentation in days."@en ;
        rdfs:label "length"@en .


###  http://ontologies.khaos.uma.es/oulad/num_of_prev_attempts
:num_of_prev_attempts rdf:type owl:DatatypeProperty ;
                      rdfs:domain :StudentInfo ;
                      rdfs:range xsd:integer ;
                      rdfs:comment "The number times the student has attempted this module."@en ;
                      rdfs:label "num_of_prev_attempts"@en .


###  http://ontologies.khaos.uma.es/oulad/region
:region rdf:type owl:DatatypeProperty ;
        rdfs:range xsd:string ;
        rdfs:comment "Identifies the geographic region, where the student lived while taking the module-presentation."@en ;
        rdfs:label "region"@en .


###  http://ontologies.khaos.uma.es/oulad/score
:score rdf:type owl:DatatypeProperty ;
       rdfs:domain :StudentAssessment ;
       rdfs:range xsd:float ;
       rdfs:comment "The student’s score in this assessment. The range is from 0 to 100. The score lower than 40 is interpreted as Fail. The marks are in the range from 0 to 100."@en ;
       rdfs:label "score"@en .


###  http://ontologies.khaos.uma.es/oulad/studied_credits
:studied_credits rdf:type owl:DatatypeProperty ;
                 rdfs:domain :StudentInfo ;
                 rdfs:range xsd:integer ;
                 rdfs:comment "The total number of credits for the modules the student is currently studying."@en ;
                 rdfs:label "studied_credits"@en .


###  http://ontologies.khaos.uma.es/oulad/sum_click
:sum_click rdf:type owl:DatatypeProperty ;
           rdfs:domain :StudentVle ;
           rdfs:range xsd:integer ;
           rdfs:comment "The number of times a student interacts with the material in that day."@en ;
           rdfs:label "sum_click"@en .


###  http://ontologies.khaos.uma.es/oulad/week_from
:week_from rdf:type owl:DatatypeProperty ;
           rdfs:domain :Vle ;
           rdfs:range xsd:integer ;
           rdfs:comment "The week from which the material is planned to be used."@en ;
           rdfs:label "week_from"@en .


###  http://ontologies.khaos.uma.es/oulad/week_to
:week_to rdf:type owl:DatatypeProperty ;
         rdfs:domain :Vle ;
         rdfs:range xsd:integer ;
         rdfs:comment "Week until which the material is planned to be used."@en ;
         rdfs:label "week_to"@en .


###  http://ontologies.khaos.uma.es/oulad/weight
:weight rdf:type owl:DatatypeProperty ;
        rdfs:domain :Assessments ;
        rdfs:range xsd:integer ;
        rdfs:comment "Weight of the assessment in %. Typically, Exams are treated separately and have the weight 100%; the sum of all other assessments is 100%"@en ;
        rdfs:label "weight"@en .


#################################################################
#    Classes
#################################################################

###  http://ontologies.khaos.uma.es/oulad/Assessments
:Assessments rdf:type owl:Class ;
             rdfs:comment "This class models the information about assessments in module-presentations. Usually, every presentation has a number of assessments followed by the final exam."@en ;
             rdfs:label "Assessments"@en .


###  http://ontologies.khaos.uma.es/oulad/Courses
:Courses rdf:type owl:Class ;
         rdfs:comment "This class models all available modules and their presentations."@en ;
         rdfs:label "Courses"@en .


###  http://ontologies.khaos.uma.es/oulad/StudentAssessment
:StudentAssessment rdf:type owl:Class ;
                   rdfs:comment "This class models the results of students’ assessments. If the student does not submit the assessment, no result is recorded."@en ;
                   rdfs:label "Student Assessment"@en .


###  http://ontologies.khaos.uma.es/oulad/StudentInfo
:StudentInfo rdf:type owl:Class ;
             rdfs:comment "This class models the demographic information about the students together with their results."@en ;
             rdfs:label "Student Info"@en .


###  http://ontologies.khaos.uma.es/oulad/StudentRegistration
:StudentRegistration rdf:type owl:Class ;
                     rdfs:comment "This class models the information about the time when the student registered for the module presentation."@en ;
                     rdfs:label "Student Registration"@en .


###  http://ontologies.khaos.uma.es/oulad/StudentVle
:StudentVle rdf:type owl:Class ;
            rdfs:comment "This class models the information about each student’s interactions with the materials in the VLE."@en ;
            rdfs:label "Student Vle"@en .


###  http://ontologies.khaos.uma.es/oulad/Vle
:Vle rdf:type owl:Class ;
     rdfs:comment "This class models the information about the available materials in the VLE. Typically these are html pages, pdf files, etc. Students have access to these materials online and their interactions with the materials are recorded."@en ;
     rdfs:label "Vle"@en .


###  Generated by the OWL API (version 5.1.18) https://github.com/owlcs/owlapi/
